rename to queue.dfy

queue.dfy
@@ -1,71 +1,203 @@
+// Trabalho 1 de Metodos Formais
+// Lucas Antunes
+// Henrique Xavier
+// Louise Dornelles
+// Gabriel Panho
+// Arthur Maia
 
-class Queue {
-    var list: array<int>;
-    var size: int;
-    var first: int;
+class {:autocontracts} Queue {
 
-    ghost var list_ghost: array<int>;
-    ghost var size_ghost: int;
+    ghost var contents: seq<int>;
 
-    // Invariant: size is non-negative
-    // Invariant: size is less than or equal to the length of list
-    // Invariant: all elements of list before index size are valid
-    // Invariant: all elements of list after index size are zero
-    predicate Valid()
-        reads *
+    var list: array<int>
+    var head: nat
+    var tail: nat
+    var size: nat
+
+    ghost predicate Valid()
     {
-        0 <= size <= list.Length
-        // forall i :: 0 <= i < size ==> list[i] |-> ? &&
-        // forall i :: size <= i < list.Length ==> list[i] == 0
+        list.Length >= 10 &&
+        size == |contents| &&
+        size <= list.Length &&
+ 
+        0 <= head < list.Length &&
+        0 <= tail < list.Length &&
+
+        (head < tail ==> size == tail - head) &&
+        (head == tail ==> size == 0 || size == list.Length) &&
+        (head > tail ==> (head + size) % list.Length == tail) &&
+        
+        contents == 
+            if size > 0 then
+                if head >= tail
+                then list[head..] + list[..tail]
+                else list[head..tail]
+            else []
     }
 
     constructor()
-        ensures Valid()
+        ensures contents == []
     {
-        list := new int[100];
+        contents := [];
+
+        list := new int[10];
+        head := 0;
+        tail := 0;
         size := 0;
-        first := 0;
     }
 
-    method enqueue(x: int)
-        requires Valid()
-        // ensures size_ghost == old(size_ghost) + 1
-        // ensures list_ghost[size_ghost - 1] == x
-        ensures Valid()
-        modifies list, this
+    method enqueue(x: int) 
+        ensures contents == old(contents) + [x]
     {
-        list[size] := x;
+        if size == list.Length {
+            grow();
+        }
+        enqueue_append(x);
+    }
+
+    method enqueue_append(x: int)
+        requires size < list.Length
+        ensures contents == old(contents) + [x]
+    {
+        list[tail] := x;
+        tail := (tail + 1) % list.Length;
         size := size + 1;
-
+        contents := contents + [x];
     }
 
-    method grow() 
-        requires Valid()
-        ensures list.Length == 2 * old(list.Length)
-        modifies this
+    method grow()
+        requires size == list.Length
+        ensures contents == old(contents)
+        ensures size == old(size)
+        ensures size < list.Length
     {
-        var new_list := new int[list.Length * 2];
+        var new_list := new int[list.Length + 10];
 
-        var i := 0;
-        while (i < size) 
-            invariant i >= 0;
-            invariant i <= size;
-            decreases size - i;
-        {
-            new_list[i] := list[i];
-            i := i + 1;
+        forall i: nat | 0 <= i < list.Length { 
+            new_list[i] := list[(head + i) % list.Length];
         }
 
         list := new_list;
+        head := 0;
+        tail := size;
+
+        Repr := {this, list};
     }
 
-    method pop() {}
+    method dequeue() returns (x: int)
+        requires |contents| > 0
+        ensures x == old(contents[0])
+        ensures contents == old(contents[1..])
+    {
+        x := list[head];
+        head := (head + 1) % list.Length;
+        size := size - 1;
+        contents := contents[1..];
+    }
 
-    method contains() {}
+    method contains(x: int) returns (r: bool)
+        ensures r <==> x in contents
+    {
+        r := if size > 0 then
+                if head >= tail
+                then x in list[head..] + list[..tail]
+                else x in list[head..tail]
+            else false;
+    }
 
-    method length() {}
+    method length() returns (l: nat) 
+        ensures l == |contents|
+    {
+        l := size;
+    }
 
-    method isEmpty() {}
+    method isEmpty() returns (r: bool)
+        ensures r <==> |contents| == 0
+    {
+        r := size == 0;
+    }
 
-    method concat() {}
+    method concat(other: Queue) returns (r: Queue)
+        requires size > 0
+        requires other.size > 0
+        requires other != this
+        requires other.Valid()
+        ensures r.contents == contents + other.contents
+    {
+        r := new Queue();
+
+        r.append(this);
+        r.append(other);
+    }
+
+    method append(other: Queue)
+        requires other != this
+        requires other.Valid()
+        ensures contents == old(contents) + other.contents
+    {
+        var i := 0;
+        while i < other.size
+            invariant other.Valid()
+            invariant Valid()
+        {
+            var x := other.peek(i);
+            enqueue(x);
+            i := i + 1;
+        }
+    }
+
+    method peek(idx: nat) returns (x: int)
+    requires size > 0
+    requires idx < size
+    ensures x == contents[idx]
+    {
+        x := list[(head + idx) % list.Length];
+    }
 }
+
+method Main()
+{
+    var q := new Queue();
+    q.enqueue(1);
+    q.enqueue(2);
+    q.enqueue(3);
+    q.enqueue(4);
+    q.enqueue(5);
+    q.enqueue(6);
+    q.enqueue(7);
+    q.enqueue(8);
+    q.enqueue(9);
+    q.enqueue(10);
+    q.enqueue(11);
+    assert q.contents == [1,2,3,4,5,6,7,8,9,10,11];
+
+    var l := q.length();
+    assert l > 10;
+
+    var deq := q.dequeue();
+    assert q.contents == [2,3,4,5,6,7,8,9,10,11];
+    assert deq == 1;
+
+    l := q.length();
+    assert l == 10;
+
+    var cnt := q.contains(5);
+    assert cnt;
+
+    cnt := q.contains(1);
+    assert !cnt;
+
+    var empty := q.isEmpty();
+    assert !empty;
+
+    var peek := q.peek(0);
+    assert peek == 2;
+
+    var q2 := new Queue();
+    q2.enqueue(12);
+    q2.enqueue(13);
+
+    var q3 := q.concat(q2);
+    assert q3.contents == [2,3,4,5,6,7,8,9,10,11,12,13];
+}
+
